
In \Section~\ref{sec:xor-games}, 
we established the connection between 
a uniform XOR target game 
(Definition~\ref{def:xor-game-uniform})
and a single epoch of our beacon protocol $\Pi_\Beacon$ 
in Definition~\ref{def:new-beacon}.
Then, in Section~\ref{sec:poisson-bernoulli}, 
we established the connection between 
$(\ell,n,\alpha)$-Poisson (resp. -Bernoulli) game 
and the beacon protocol 
under a private (resp. public) leader election scheme 
(Section~\ref{sec:leader-election-public-private})
where the total adversarial probability is $\alpha$. 
Section~\ref{sec:poisson-bernoulli} 
culminated in tail bounds 
on the grinding power in those games; 
see Lemma~\ref{lemma:xor-game-poisson-gamma} and ~\ref{lemma:xor-game-Bernoulli-gamma}. 
Finally, recall from Fact~\ref{fact:min-entropy-grinding-power} 
that the min-entropy loss in any beacon no more than the logarithm of its grinding power. 

In this \Section, we connect these ideas
to prove tail bounds for the min-entropy loss in the beacon output in a single epoch. 
Then we use the iterative beacon lemma (Lemma~\ref{lemma:beacon-composition}) 
to argue that over an execution spanning $L$ epochs, 
the same upper bound holds but the failure probability is inflated by 
a multiplicative factor of the grinding power.



\section{Grinding power in a single epoch}



\begin{lemma}[Adaptive adversary, single epoch]\label{lemma:beacon-poisson-single-epoch}
  Let $\alpha \in (0, 1)$ and suppose it satisfies \eqref{eq:alphatothen-epsp}.
  Let $f(\alpha)$ and $\rho$ be as in \eqref{eq:f-poisson} and \eqref{eq:rho-poisson}.
  Let $\Pi_\Beacon$ be a $(T,k,s,d,\PrivateLeaderElection(\alpha), \EpsP)$-beacon 
  where $d$ is from~\eqref{eq:d-multiepoch}.
  Let $\eta$ be the beacon output after the first epoch. 
  Then 
  \begin{equation}\label{eq:security-poisson-single-epoch}
    \Pr_{\PrivateLeaderElection{\alpha}}\left[\MinEntropy(\eta) \geq \kappa - \rho \right] \geq 1 - 3 \EpsP
    \,.
  \end{equation}
\end{lemma}

\begin{proof}  
  Consider Lemma~\ref{lemma:xor-game-poisson-gamma} 
  with $\ell = k/d$ and $n = (T-k)/d$. 
          % \gamma = \left(\frac{n^{1 + \lambda} }{ (1+\alpha) \EpsP} \right)^{1/\lambda}
          %     \cdot \begin{cases}
          %         (1 + 3 \alpha + \alpha^2)^{\ell/\lambda} &\quad\text{if $\alpha \leq 0.41$\,,} \\
          %         (1/\alpha)^{\ell/\lambda} &\quad\text{otherwise\,.}
          %     \end{cases}
  The total failure probability, 
  considering both $\Pr[g \geq \gamma]$ and 
  the $(\EpsP, k, s)$-secure protocol $\Blockchain$, 
  is $(\alpha^n + \EpsP) + \EpsP$. 
  Since we assume~\eqref{eq:alphatothen-epsp}, it is at most $3 \EpsP$.

  Recall $\lambda$ from~\eqref{eq:lambda-star-poisson} and $\gamma$ from~\eqref{eq:xor-poisson-tail-gamma}.

  \Paragraph{Case: $\alpha \leq 0.41$.}
  In this case, $\lambda = 2$ and 
  the min-entropy loss, 
  \begin{align*}
    \rho &= \log_2(\gamma) \\
        &= \log_2 \left[  \left(\frac{n^{1 + \lambda} }{ (1+\alpha) \EpsP} \right)^{1/\lambda}
          \cdot (1 + 3 \alpha + \alpha^2)^{\ell/\lambda}
        \right] \\
        &= (1/2)\log_2 \left(\frac{n^3}{ (1+\alpha) \EpsP} \right) 
          + (\ell/2) \log_2(1 + 3 \alpha + \alpha^2)
        \,.
  \end{align*}
  
  \Paragraph{Case: $\alpha > 0.41$.}
  In this case, $\lambda = 2 \ln(1/\alpha)/\ln(1+3\alpha+\alpha^2) = 2/f(\alpha)$ and 
  the min-entropy loss, 
  \begin{align*}
    \rho &= \log_2(\gamma) \\
        &= \log_2 \left[  \left(\frac{n^{1 + \lambda} }{ (1+\alpha) \EpsP} \right)^{1/\lambda}
          \cdot (1/\alpha)^{\ell/\lambda}
        \right] \\
        &= (1/\lambda) \log_2 \left(\frac{n^{1 + \lambda} }{ (1+\alpha) \EpsP} \right)
          + (\ell/\lambda) \log_2(1/\alpha)
        \\
        &= (f(\alpha)/2)\log_2 \left(\frac{n^{(1 + 2/f(\alpha))} }{ (1+\alpha) \EpsP} \right) 
          + (\ell f(\alpha)/2) \log_2(1/\alpha)
          \\
        &= (f(\alpha)/2)\log_2 \left(\frac{n^{1 + 2/f(\alpha)} }{ (1+\alpha) \EpsP} \right) 
          + (\ell/2) \log_2(1 + 3\alpha + \alpha^2)
        \,.
  \end{align*}

  Finally, notice that in the expression of $\rho$, we can have
  $$
  (\ell/2) \log_2(1+3\alpha + \alpha^2) = \frac{k}{T-k} \cdot \frac{f(\alpha)}{2}\cdot \log_2(1/\EpsP)
  $$
  using $\ell = k/d$ and taking $d$ from~\eqref{eq:d-multiepoch}.
\end{proof}
% \hfill\qed

\begin{lemma}[Static adversary, single epoch]\label{lemma:beacon-bernoulli-single-epoch}
  Let $\alpha \in (0, 0.41)$ and suppose it satisfies \eqref{eq:alphatothen-epsp}.
  Let $f(\alpha)$ and $\rho$ be as in \eqref{eq:f-bernoulli} and \eqref{eq:rho-bernoulli}.
  Let $\Pi_\Beacon$ be a $(T,k,s,d,\PublicLeaderElection(\alpha), \EpsP)$-beacon.
  Let $\eta$ be the beacon output after the first epoch. 
  Then 
  \begin{equation}\label{eq:security-bernoulli-single-epoch}
    \Pr_{\PublicLeaderElection{\alpha}}\left[\MinEntropy(\eta) \geq \kappa - \rho \right] \geq 1 - 3 \EpsP
    \,.
  \end{equation}
\end{lemma}
\begin{proof}  
  Consider Lemma~\ref{lemma:xor-game-Bernoulli-gamma} 
  with $\ell = k/d$ and $n = (T-k)/d$. 
  The min-entropy loss, 
  \begin{align*}
    \rho &= \log_2(\gamma) \\
        &= \log_2 \left[  2^{\ell + 1} \left(
                \frac{n}{(1+\alpha)\EpsP}
            \right)^{1/\log_2(1/\alpha)}\right] \\
        &= \ell + 1 + f(\alpha) \log_2\left(\frac{n}{(1+\alpha)\EpsP}\right)
        \,.
  \end{align*}
  The total failure probability, 
  considering both $\Pr[g \geq \gamma]$ and 
  the $(\EpsP, k, s)$-secure protocol $\Blockchain$, 
  is $(\alpha^n + \EpsP) + \EpsP$. 
  Since we assume~\eqref{eq:alphatothen-epsp}, it is at most $3 \EpsP$.
\end{proof}
% \hfill\qed



\section{Grinding power over multiple epochs; proof of main theorems}

In this section, we build upon the results of the previous section 
and apply the composition lemma (Lemma~\ref{lemma:beacon-composition}). 
This would give us tail bounds for an iterated beacon.



\subsection*{Proof of Theorem~\ref{thm:beacon-poisson-multi-epoch}}
% \begin{proof}
  Consider Lemma~\ref{lemma:xor-game-poisson-gamma}, 
  with $\ell = k/d$ and $n = (T-k)/d$, 
  in conjunction with Lemma~\ref{lemma:beacon-composition}.
  It follows that the min-entropy loss, $\rho$, 
  would be same as in the single-epoch case, 
  given by Lemma~\ref{lemma:beacon-poisson-single-epoch} 
  for $\alpha \leq 0.41$. 
  Recall $\lambda$ from~\eqref{eq:lambda-star-poisson} and $\gamma$ from~\eqref{eq:xor-poisson-tail-gamma}.
  Since $\alpha \leq 0.41$, $\lambda = 2$.
  
  Let us write $a = 1 + 3 \alpha + \alpha^2$ 
  % $$
 %    a = 
 %      % \begin{cases}
 %        1 + 3 \alpha + \alpha^2 &\quad\text{if $\alpha \leq 0.41$\,,} \\
 %        1/\alpha &\quad\text{otherwise\,,}
 %    \end{cases}
  % $$
  and 
  $$
    p(d) = n^{1+1/\lambda} \EpsP^{1 - 1/\lambda} a^{\ell/\lambda}
    \,.
  $$
  Then, according to Lemma~\ref{lemma:beacon-composition}, 
  the min-entropy loss is at most $\log_2(\gamma)$ 
  except with probability at most $3 L p(d)$. 
  Let $\delta \in (0, 1)$ so that $p(d) \leq \EpsP^\delta$; 
  the value of $\delta$ will be determined later. 
  We wish to select a $d$ so that $\delta$ is maximized.

  First, we require that 
  \begin{align*}
    &\alpha^n \leq \EpsP\,,\\
    \text{or}\quad &
      1/\EpsP \leq (1/\alpha)^{(T - k)/d}\,,\\
    \text{or}\quad &
      \log_2(1/\EpsP) \leq ((T - k)/d)\log_2(1/\alpha)\,,\\
    \text{or}\quad &
      d \leq \dMax \triangleq \frac{(T - k)\log_2(1/\alpha)}{\log_2(1/\EpsP)}
      \,.
  \end{align*}

  We also want 
  \begin{align*}
    &p(d) \leq \EpsP^{\delta}\,,\\
    \text{or}\quad &
      n^{1+1/\lambda} \EpsP^{1 - 1/\lambda} a^{\ell/\lambda} \leq \EpsP^\delta \,,\\
    \text{or}\quad &
      (1+1/\lambda)\log_2(n)
      + (1/\lambda - 1)\log_2(1/\EpsP) 
      + (\ell/\lambda) \log_2(a) \leq -\delta \log_2(1/\EpsP) \,,\\
    \text{or}\quad &      
      (\ell/\lambda) \log_2(a) \leq (1-\delta - 1/\lambda) \log_2(1/\EpsP) - (1+1/\lambda)\log_2(n)\,,\\
    \text{or}\quad &      
      (k/d\lambda) \log_2(a) \leq (1-\delta - 1/\lambda) \log_2(1/\EpsP) - (1+1/\lambda)\log_2((T-k)/d)\,,\\
    \text{or}\quad &      
      \frac{(k/\lambda) \log_2(a)}{(1-\delta - 1/\lambda) \log_2(1/\EpsP) - (1+1/\lambda)\log_2((T-k)/d)} \leq d
      \,.
  \end{align*}
  
  For the above inequality to hold, 
  it suffices to take $d \geq \dMin(\delta)$ where 
  $$
    \dMin(\delta) = \frac{(k/\lambda) \log_2 a}{(1 - \delta - 1/\lambda) \log_2(1/\EpsP) - (1+1/\lambda) \log_2(T - k)}
    \,.
  $$
  An admissible $d$ must satisfy
  \begin{align*}
    &\dMin(\delta) \leq \dMax \,,\\
    \text{or}\quad &      
      \frac{(k/\lambda) \log_2 a}{(1 - \delta - 1/\lambda) \log_2(1/\EpsP) - (1+1/\lambda) \log_2(T - k)}
        \leq (T - k) \log_2(1/\alpha)/\log_2(1/\EpsP) \,,\\
    \text{or}\quad &      
      \frac{(k/\lambda) \log_2 a}{(T - k) \log_2(1/\alpha)/\log_2(1/\EpsP)} 
        \leq (1 - \delta - 1/\lambda) \log_2(1/\EpsP) - (1+1/\lambda) \log_2(T - k) \,,\\
    \text{or}\quad &      
      \frac{(k/\lambda) \log_2 a}{(T - k) \log_2(1/\alpha)} + \frac{(1+1/\lambda) \log_2(T - k)}{\log_2(1/\EpsP)}
        \leq 1 - \delta - 1/\lambda  \,,\\
    \text{or}\quad &      
      \frac{k}{T-k}\cdot \frac{f(\alpha)}{\lambda} + (1+1/\lambda) \frac{ \log_2(T - k)}{\log_2(1/\EpsP)}
        \leq 1 - \delta - 1/\lambda  \,,
  %       \\
    % \text{or}\quad &      
    %   \frac{(1/\lambda) \log_2 a}{(R - 1) \log_2(1/\alpha)} + \frac{(1+1/\lambda) \log_2(k(R-1))}{\log_2(1/\EpsP)}
    %     \leq 1 - \delta - 1/\lambda  
        \,.
  \end{align*}
  where we used $f(\alpha) = \log_2(a)/\log_2(1/\alpha)$. 
  Thus, if we take $d = \lfloor \dMax \rfloor$, we can achieve  $p(d) \leq \EpsP^{\delta}$ 
  where 
  \begin{align}
    \delta
      % &\leq \leq 1 - 1/\lambda - \frac{(1/\lambda) \log_2 a}{(R-1) \log_2(1/\alpha)} - \frac{(1+1/\lambda) \log_2(k(R-1))}{\log_2(1/\EpsP)}  \\
      &\leq 1 - 1/\lambda - \frac{k}{T-k}\cdot \frac{f(\alpha)}{\lambda} - (1+1/\lambda) \frac{ \log_2(T - k)}{\log_2(1/\EpsP)}\,. \label{eq:delta}    
  \end{align}


  \begin{fact*}
    If $x,y \in \RR$ satisfy $y = x^{-1/\log_2(1/x)}$ then $y = 2$.
  \end{fact*}
  \noindent
  For further simplification, let us use the assumption that $\alpha \leq 0.41$ 
  and write $c = k/(T-k)$; 
  this implies $\lambda = 2$, 
  \begin{align*}
    \delta
      &\leq \frac{1}{2} - \frac{c f(\alpha)}{2} - \frac{3}{2} \frac{ \log_2(T - k)}{\log_2(1/\EpsP)}\,, 
      \qquad \text{and}\\
    \EpsP^\delta  
      &\leq \EpsP^{1/2 - c f(\alpha)/2} \cdot \left[ \EpsP^{-1/\log_2(1/\EpsP)} \right]^{(3/2)\log_2(T - k)} \\
      &= \EpsP^{1/2 - c f(\alpha)/2} \cdot 2^{(3/2)\log_2(T - k)} \qquad\text{Using above Fact with $x = \EpsP$}\\
      &= \EpsP^{1/2 - (k/(T-k)) f(\alpha)/2} \cdot (T - k)^{3/2} 
      \,,
  \end{align*}
  as claimed in the theorem statement. 
% \end{proof}
\hfill\qed


\subsection*{Proof of Theorem~\ref{thm:beacon-bernoulli-multi-epoch}}
% \begin{proof}
  Consider Lemma~\ref{lemma:xor-game-Bernoulli-gamma}, 
  with $\ell = k/d$ and $n = (T-k)/d$, 
  in conjunction with Lemma~\ref{lemma:beacon-composition}.
  It follows that the min-entropy loss, $\rho$, 
  would be same as in the single-epoch case, 
  given by Lemma~\ref{lemma:beacon-bernoulli-single-epoch}.

  The failure probability, however, would be at most
  \begin{align*}
    3 L 2^\rho \EpsP
    &= 3 L 2^{\ell + 1} 
      \left(\frac{n}{1+\alpha}\right)^{f(\alpha)} 
      \EpsP^{1 - f(\alpha)}
      \,.
  \end{align*}
  
% \end{proof}
\hfill\qed